Add top-level spec for rsc and use KObject in the model

src/verification/model.v
@@ -1,11 +1,48 @@
-From Perennial.algebra Require Import auth_map.
-From New.proof.github_com.goose_lang.goose.model.channel Require Import auth_set.
+From Perennial.algebra Require Export auth_map.
+From New.proof.github_com.goose_lang.goose.model.channel Require Export auth_set.
 Require Import New.proof.sync.
 From verification.k8s_io.api.core Require Export v1_init.
+From verification.k8s_io.api.apps Require Import v1_init.
+
+Module KKind.
+  Inductive t :=
+  | Pod
+  | ReplicaSet.
+
+  Definition encode (k : t) : nat :=
+    match k with
+    | Pod => 0
+    | ReplicaSet => 1
+    end.
+
+  Definition decode (n : nat) : t :=
+    match n with
+    | 0%nat => Pod
+    | _ => ReplicaSet
+    end.
+
+  Lemma decode_encode k : decode (encode k) = k.
+  Proof. destruct k; reflexivity. Qed.
+
+  Global Instance eq_dec : EqDecision t.
+  Proof. solve_decision. Qed.
+
+  Global Instance countable : Countable t.
+  Proof.
+    refine (inj_countable' encode decode _).
+    intros []; apply decode_encode.
+  Qed.
+End KKind.
+
+Module KObject.
+  Inductive t :=
+  | Pod (p : v1.Pod.t)
+  | ReplicaSet (rs : v1.ReplicaSet.t).
+End KObject.
 
 Module KKey.
   Record t := mk {
-    kind : go_string;
+    kind : KKind.t;
     namespace : go_string;
     name : go_string
   }.
@@ -17,7 +54,7 @@ Module KKey.
   Proof.
     refine (inj_countable'
               (fun k => (kind k, namespace k, name k))
-              (fun '(k, ns, n) => mk k ns n)
+              (fun '(k, ns, n) => mk  k ns n)
               _).
     intros []; reflexivity.
   Qed.
@@ -28,12 +65,12 @@ Global Existing Instance KKey.countable.
 
 Section model.
 
-Context `{!mapG Σ KKey.t v1.Pod.t}.
+Context `{!mapG Σ KKey.t KObject.t}.
 Context `{!mapG Σ KKey.t (gset KKey.t)}.
 Context `{!auth_setG Σ KKey.t}.
 Context `{heapGS Σ, !ffi_semantics _ _}.
 
-Definition foo γ (m : gmap KKey.t v1.Pod.t) k v : iProp Σ :=
+Definition foo γ (m : gmap KKey.t KObject.t) k v : iProp Σ :=
   map_ctx γ 1 m ∗ k [[ γ ]]↦ v.
 
 Definition bar γ (m : gmap KKey.t (gset KKey.t)) k v : iProp Σ :=
@@ -42,25 +79,22 @@ Definition bar γ (m : gmap KKey.t (gset KKey.t)) k v : iProp Σ :=
 Definition baz γ (s : gset KKey.t) (v : KKey.t) : iProp Σ :=
   auth_set_auth γ s ∗ auth_set_frag γ v.
 
-Axiom state_well_formed : gmap KKey.t v1.Pod.t → Prop.
+Axiom kubernetes_state_well_formed : gmap KKey.t KObject.t → Prop.
 
-Axiom state_and_children_consistent : gmap KKey.t v1.Pod.t → gmap KKey.t (gset KKey.t) → Prop.
+Axiom kubernetes_state_consistent : gmap KKey.t KObject.t → gmap KKey.t (gset KKey.t) → gset KKey.t → Prop.
 
-Axiom state_and_fresh_keys_consistent : gmap KKey.t v1.Pod.t → gset KKey.t → Prop.
+Definition is_kubernetes_state_inner γ_state γ_children γ_fresh_keys : iProp Σ :=
+  ∃ (m_state : gmap KKey.t KObject.t) (m_children : gmap KKey.t (gset KKey.t)) (s_fresh_keys : gset KKey.t),
+    "Hstate" ∷ map_ctx γ_state 1 m_state ∗
+    "Hchildren" ∷ map_ctx γ_children 1 m_children ∗
+    "Hfreshkeys" ∷ auth_set_auth γ_fresh_keys s_fresh_keys ∗
+    "%Hwellformed" ∷ ⌜ kubernetes_state_well_formed m_state ⌝ ∗
+    "%Hconsistent" ∷ ⌜ kubernetes_state_consistent m_state m_children s_fresh_keys ⌝.
 
-Definition is_kubernetes_state_inner γ : iProp Σ :=
-  ∃ (m_state : gmap KKey.t v1.Pod.t) (m_children : gmap KKey.t (gset KKey.t)) (s_fresh_keys : gset KKey.t),
-    map_ctx γ 1 m_state ∗
-    map_ctx γ 1 m_children ∗
-    auth_set_auth γ s_fresh_keys ∗
-    ⌜ state_well_formed m_state ∧
-      state_and_children_consistent m_state m_children ∧
-      state_and_fresh_keys_consistent m_state s_fresh_keys ⌝.
+Definition is_kubernetes_state γ_state γ_children γ_fresh_keys : iProp Σ :=
+  ∃ l, "#Hkinv" ∷ is_Mutex l (is_kubernetes_state_inner γ_state γ_children γ_fresh_keys).
 
-Definition is_kubernetes_state γ : iProp Σ :=
-  ∃ l, is_Mutex l (is_kubernetes_state_inner γ).
-
-Global Instance is_kubernetes_state_persistent γ : Persistent (is_kubernetes_state γ).
+Global Instance is_kubernetes_state_persistent γ_state γ_children γ_fresh_keys : Persistent (is_kubernetes_state γ_state γ_children γ_fresh_keys).
 Proof. apply _. Qed.
 
 End model.
